DS/Heap.v
@@ -1,0 +1,81 @@
+Require Export Tree.
+
+Inductive isHeap {A : Type} (R : A -> A -> Prop) : Tree A -> Prop :=
+    | isHeap_E : isHeap R E
+    | isHeap_T :
+        forall (v : A) (l : list (Tree A)),
+          Forall (fun t : Tree A => forall x : A, Elem x t -> R v x) l ->
+          Forall (isHeap R) l ->
+            isHeap R (T v l).
+
+Hint Constructors isHeap : core.
+
+Ltac isHeap :=
+repeat match goal with
+    | H : isHeap _ E        |- _ => clear H
+    | H : isHeap _ (T _ _)  |- _ => inv H
+    | H : Forall _ []       |- _ => clear H
+    | H : Forall _ (_ :: _) |- _ => inv H
+    |                       |- isHeap _ E      => constructor
+    |                       |- isHeap _ _ -> _ => intro
+    |                       |- Forall _ _ -> _  => intro
+end; auto.
+
+Ltac isHeap' :=
+repeat match goal with
+    | H : isHeap _ E        |- _ => clear H
+    | H : isHeap _ (T _ _)  |- _ => inv H
+    | H : Forall _ []       |- _ => clear H
+    | H : Forall _ (_ :: _) |- _ => inv H
+    |                       |- isHeap _ E       => constructor
+    |                       |- isHeap _ (T _ _) => constructor
+    |                       |- Forall _ []       => constructor
+    |                       |- Forall _ (_ :: _) => constructor
+    |                       |- isHeap _ _ -> _  => intro
+    |                       |- Forall _ _ -> _  => intro
+end; eauto.
+
+Inductive OK {A : Type} (R : A -> A -> Prop) (x : A) : Tree A -> Prop :=
+    | OK_E : OK R x E
+    | OK_N :
+        forall (v : A) (l : list (Tree A)),
+          R x v -> OK R x (T v l).
+
+Inductive isHeap2 {A : Type} (R : A -> A -> Prop) : Tree A -> Prop :=
+    | isHeap2_E : isHeap2 R E
+    | isHeap2_T :
+        forall (v : A) (l : list (Tree A)),
+          Forall (fun t : Tree A => OK R v t) l ->
+            Forall (isHeap2 R) l -> isHeap2 R (T v l).
+
+Hint Constructors isHeap OK isHeap2 : core.
+
+Ltac isHeap2 :=
+repeat match goal with
+    | H : isHeap2 _ E       |- _ => clear H
+    | H : isHeap2 _ (T _ _) |- _ => inv H
+    | H : Forall _ []       |- _ => clear H
+    | H : Forall _ (_ :: _) |- _ => inv H
+    |                       |- isHeap2 _ E      => constructor
+    |                       |- isHeap2 _ _ -> _ => intro
+    |                       |- Forall _ _ -> _  => intro
+end; auto.
+
+Ltac isHeap2' :=
+repeat match goal with
+    | H : isHeap2 _ E       |- _ => clear H
+    | H : isHeap2 _ (T _ _) |- _ => inv H
+    | H : Forall _ []       |- _ => clear H
+    | H : Forall _ (_ :: _) |- _ => inv H
+    |                       |- isHeap2 _ E       => constructor
+    |                       |- isHeap2 _ (T _ _) => constructor
+    |                       |- Forall _ []       => constructor
+    |                       |- Forall _ (_ :: _) => constructor
+    |                       |- isHeap2 _ _ -> _  => intro
+    |                       |- Forall _ _ -> _  => intro
+end; eauto.
+
+Lemma isHeap_isEmpty :
+  forall (A : Type) (R : A -> A -> Prop) (t : Tree A),
+    isEmpty t = true -> isHeap R t.
+Proof. Tree_ind. Qed.
